Added new interface and proofs

mrdts-new/Observed-remove_set_eff/App_new.fst
@@ -7,35 +7,26 @@ module M = Map_extended
 
 let cf = (int * bool)
 
-// concrete state of ew flag
-type concrete_st_e = M.t nat cf // (replica_id, ctr, flag) //replica ids are unique
-
 // the concrete state type
-type concrete_st = M.t nat concrete_st_e // element ->
+type concrete_st = M.t nat (M.t nat cf) // element ->
                                        //    replica ID -> 
                                        //       (ctr, flag) //elements & replica ids are unique
 
-// init state of ew flag
-let init_st_e : concrete_st_e = M.const (0, false)
-
 // init state
-let init_st : concrete_st = M.const init_st_e
-
-let sel_e (s:concrete_st) e = if M.contains s e then M.sel s e else (M.const (0, false))
+let init_st : concrete_st = M.const (M.const (0, false))
 
 let sel_id (s:M.t nat cf) id = if M.contains s id then M.sel s id else (0, false)
 
-let ele_id (s:concrete_st) (e id:nat) =
-  M.contains s e /\ M.contains (sel_e s e) id
+let sel (s:concrete_st) e = if M.contains s e then M.sel s e else (M.const (0, false))
 
 // equivalence relation of ew flag
-let eq_e (a b:concrete_st_e) =
-  (forall id. (M.contains a id = M.contains b id) /\ (sel_id a id == sel_id b id))
-
+let eq_e (a b:M.t nat cf) =
+  (forall id. M.contains a id = M.contains b id /\ sel_id a id = sel_id b id)
+  
 // equivalence between 2 concrete states
 let eq (a b:concrete_st) =
-  (forall e. M.contains a e = M.contains b e) /\
-  (forall e. M.contains a e ==> eq_e (sel_e a e) (sel_e b e))
+ (forall e. M.contains a e = M.contains b e /\ eq_e (sel a e) (sel b e))
+ //(forall k. (M.contains a k = M.contains b k) /\ eq_e (sel a k) (sel b k)) 
 
 let symmetric (a b:concrete_st) 
   : Lemma (requires eq a b)
@@ -58,15 +49,15 @@ let get_ele (o:op_t) : nat =
   match snd (snd o) with
   |Add e -> e
   |Rem e -> e
-  
+
 // apply an operation to a state
 let do (s:concrete_st) (o:op_t) : concrete_st =
  match o with
-  |(_, (rid, Add e)) -> M.upd s e (M.upd (sel_e s e) rid (fst (sel_id (sel_e s e) rid) + 1, true))
+  |(_, (rid, Add e)) -> M.upd s e (M.upd (sel s e) rid (fst (sel_id (sel s e) rid) + 1, true))
   |(_, (rid, Rem e)) -> M.iter_upd (fun k v -> if k = e then ((M.map_val (fun (c,f) -> (c, false))) v) else v) s
-
+ 
 //conflict resolution
-let rc (o1:op_t) (o2:op_t(*{distinct_ops o1 o2}*)) =
+let rc (o1 o2:op_t) =  
   match snd (snd o1), snd (snd o2) with
   |Add e1, Rem e2 -> if e1 = e2 then Snd_then_fst else Either
   |Rem e1, Add e2 -> if e1 = e2 then Fst_then_snd else Either
@@ -97,38 +88,32 @@ let merge_ew (l a b:(M.t nat cf)) : (M.t nat cf) =
 let merge (l a b:concrete_st) : concrete_st =
   let eles = S.union (M.domain l) (S.union (M.domain a) (M.domain b)) in
   let u = M.const_on eles init_st in
-  M.iter_upd (fun k v -> merge_ew (sel_e l k) (sel_e a k) (sel_e b k)) u
+  M.iter_upd (fun k v -> merge_ew (sel l k) (sel a k) (sel b k)) u
 
 /////////////////////////////////////////////////////////////////////////////
 
+let rc_non_comm_help1 (o1 o2:op_t)
+  : Lemma (ensures (((Add? (snd (snd o1)) /\ Rem? (snd (snd o2))) \/ (Rem? (snd (snd o1)) /\ Add? (snd (snd o2)))) /\ get_ele o1 = get_ele o2)
+  ==> ~ (eq (do (do init_st o1) o2) (do (do init_st o2) o1))) = ()
+
+let rc_non_comm (o1 o2:op_t)
+  : Lemma (ensures Either? (rc o1 o2) <==> commutes_with o1 o2) = 
+  rc_non_comm_help1 o1 o2
+  
 let no_rc_chain (o1 o2 o3:op_t)
   : Lemma (ensures ~ (Fst_then_snd? (rc o1 o2) /\ Fst_then_snd? (rc o2 o3))) = ()
 
-let relaxed_comm (s:concrete_st) (o1 o2 o3:op_t)
+let cond_comm_base (s:concrete_st) (o1 o2 o3:op_t) 
   : Lemma (requires Fst_then_snd? (rc o1 o2) /\ ~ (Either? (rc o2 o3)))
           (ensures eq (do (do (do s o1) o2) o3) (do (do (do s o2) o1) o3)) = ()
 
-let non_comm (o1 o2:op_t)
-  : Lemma (ensures Either? (rc o1 o2) <==> commutes_with o1 o2) =
-  assert (((Add? (snd (snd o1)) /\ Rem? (snd (snd o2)) /\ get_ele o1 = get_ele o2) \/ 
-           (Rem? (snd (snd o1)) /\ Add? (snd (snd o2)) /\ get_ele o1 = get_ele o2)) ==>
-           ~ (eq (do (do init_st o1) o2) (do (do init_st o2) o1))); ()
-         
-let cond_comm (o1:op_t) (o2:op_t{~ (Either? (rc o1 o2))}) (o3:op_t) =
-  if Rem? (snd (snd o3)) && get_ele o1 = get_ele o3 then true else false
-
-#push-options "--z3rlimit 100 --max_ifuel 3 --split_queries on_failure"
-let cond_comm_base (s:concrete_st) (o1 o2 o3:op_t)
-  : Lemma (requires distinct_ops o1 o2 /\ ~ (Either? (rc o1 o2)) /\ cond_comm o1 o2 o3)
-          (ensures eq (do (do (do s o1) o2) o3) (do (do (do s o2) o1) o3)) = ()
-
-let cond_comm_ind (s:concrete_st) (o1 o2 o3 o:op_t) (l:log)
-  : Lemma (requires distinct_ops o1 o2 /\ ~ (Either? (rc o1 o2)) /\ cond_comm o1 o2 o3 /\
+#set-options "--z3rlimit 300 --ifuel 4"
+let cond_comm_ind (s:concrete_st) (o1 o2 o3 o:op_t) (l:seq op_t)
+  : Lemma (requires Fst_then_snd? (rc o1 o2) /\ ~ (Either? (rc o2 o3)) /\
                     eq (do (apply_log (do (do s o1) o2) l) o3) (do (apply_log (do (do s o2) o1) l) o3))
           (ensures eq (do (do (apply_log (do (do s o1) o2) l) o) o3) (do (do (apply_log (do (do s o2) o1) l) o) o3)) = ()
-          
-/////////////////////////////////////////////////////////////////////////////
 
+/////////////////////////////////////////////////////////////////////////////
 // Merge commutativity
 let merge_comm (l a b:concrete_st)
    : Lemma (ensures (eq (merge l a b) (merge l b a))) = ()
@@ -137,466 +122,72 @@ let merge_comm (l a b:concrete_st)
 let merge_idem (s:concrete_st)
    : Lemma (ensures eq (merge s s s) s) = ()
 
-(*Two OP RC*)
-//////////////// 
-let rc_ind_right' (l a b:concrete_st) (o1 o2' o2:op_t)
-   : Lemma (requires Fst_then_snd? (rc o1 o2) /\
-                     eq (merge l (do a o1) (do b o2)) (do (merge l (do a o1) b) o2) /\
-                     (forall e. eq_e (sel_e (merge l (do a o1) (do (do b o2') o2)) e) (sel_e (do (merge l (do a o1) (do b o2')) o2) e)))
-           (ensures eq (merge l (do a o1) (do (do b o2') o2)) (do (merge l (do a o1) (do b o2')) o2)) = ()
+///////////////////////////////////////////////////////////////////////////
 
-let rc_ind_left' (l a b:concrete_st) (o1 o1' o2:op_t)
-  : Lemma (requires Fst_then_snd? (rc o1 o2) /\
-                    eq (merge l (do a o1) (do b o2)) (do (merge l (do a o1) b) o2) /\
-                    (forall e. eq_e (sel_e (merge l (do (do a o1') o1) (do b o2)) e) (sel_e (do (merge l (do (do a o1') o1) b) o2) e)))
-          (ensures eq (merge l (do (do a o1') o1) (do b o2)) (do (merge l (do (do a o1') o1) b) o2)) = ()
+let base_2op o1 o2 = ()
 
-//Special case of rc_intermediate_v1
-let rc_ind_lca' (l:concrete_st) (o o1 o2:op_t)
-  : Lemma (requires Fst_then_snd? (rc o1 o2) /\ 
-                    eq (merge l (do l o1) (do l o2)) (do (do l o1) o2) /\
-                    (forall e. eq_e (sel_e (merge (do l o) (do (do l o) o1) (do (do l o) o2)) e) (sel_e (do (do (do l o) o1) o2) e)))
-          (ensures eq (merge (do l o) (do (do l o) o1) (do (do l o) o2)) (do (do (do l o) o1) o2)) = ()
+let ind_lca_2op l o1 o2 ol = ()
 
-let rc_base' (o1 o2:op_t)
-  : Lemma (requires Fst_then_snd? (rc o1 o2))
-          (ensures eq (merge init_st (do init_st o1) (do init_st o2)) (do (do init_st o1) o2)) = ()
+let inter_right_base_2op_fts (l a b :concrete_st) (o1 o2 ob ol:op_t)
+  : Lemma (requires Fst_then_snd? (rc o2 o1) /\ get_rid o1 <> get_rid o2 /\ Fst_then_snd? (rc ob ol) /\ get_rid ob <> get_rid ol /\
+                    eq (merge l (do a o1) (do (do b ob) o2)) (do (merge l a (do (do b ob) o2)) o1) /\ //from ind_right_2op
+                    eq (merge (do l ol) (do (do a ol) o1) (do (do b ol) o2)) (do (merge (do l ol) (do a ol) (do (do b ol) o2)) o1))
+          (ensures eq (merge (do l ol) (do (do a ol) o1) (do (do (do b ob) ol) o2)) (do (merge (do l ol) (do a ol) (do (do (do b ob) ol) o2)) o1)) = ()
 
-(*let aux (l s1 s2 s3:concrete_st) (o o' o1' o1 o2:op_t)
-  : Lemma (requires distinct_ops o o' /\ Fst_then_snd? (rc o o') /\
-                    distinct_ops o1 o2 /\ Fst_then_snd? (rc o1 o2) /\
-                    distinct_ops o1' o' /\ Fst_then_snd? (rc o1' o') /\
-                    eq (merge (do l o') (do (do s1 o') o1) (do (do s2 o') o2)) (do (do (do s3 o') o1) o2) /\
-                    eq (merge l (do s1 o1) (do s2 o2)) (do (do s3 o1) o2))
-          (ensures forall e. eq_e (sel_e (merge (do l o') (do (do (do s1 o1') o') o1) (do (do (do s2 o) o') o2)) e)
-                                    (sel_e (do (do (do (do (do s3 o1') o) o') o1) o2) e)) =
-  if get_ele o2 = get_ele o' && get_rid o2 = get_rid o' then admit() //done
-  else if get_ele o2 = get_ele o' && get_rid o2 <> get_rid o' then admit() //done
-  else if get_ele o2 <> get_ele o' && get_rid o2 = get_rid o' then admit() //done
-  else admit()*)
-  
-let rc_intermediate_base_right' (l s1 s2 s3:concrete_st) (o o' o1 o2:op_t) 
-  : Lemma (requires distinct_ops o o' /\ Fst_then_snd? (rc o o') /\ 
-                    distinct_ops o1 o2 /\ Fst_then_snd? (rc o1 o2) /\
-                    eq (merge (do l o') (do (do s1 o') o1) (do (do s2 o') o2)) (do (do (do s3 o') o1) o2) /\
-                    eq (merge l (do s1 o1) (do s2 o2)) (do (do s3 o1) o2) /\
-                    eq (merge l (do s1 o') (do s2 o)) (do (do s3 o) o') /\ //***EXTRA***
-                    (forall e. eq_e (sel_e (merge (do l o') (do (do s1 o') o1) (do (do (do s2 o) o') o2)) e)
-                               (sel_e (do (do (do (do s3 o) o') o1) o2) e)))
-          (ensures eq (merge (do l o') (do (do s1 o') o1) (do (do (do s2 o) o') o2)) (do (do (do (do s3 o) o') o1) o2)) = ()
-  (*if get_ele o2 = get_ele o' && get_rid o2 = get_rid o' then () //done
-  else if get_ele o2 = get_ele o' && get_rid o2 <> get_rid o' then () //done
-  else if get_ele o2 <> get_ele o' && get_rid o2 = get_rid o' then () //done
-  else () //done*)
-
-let rc_intermediate_base_left' (l s1 s2 s3:concrete_st) (o o' o1 o2:op_t) 
-  : Lemma (requires distinct_ops o o' /\ Fst_then_snd? (rc o o') /\ 
-                    distinct_ops o1 o2 /\ Fst_then_snd? (rc o1 o2) /\
-                    eq (merge (do l o') (do (do s1 o') o1) (do (do s2 o') o2)) (do (do (do s3 o') o1) o2) /\
-                    eq (merge l (do s1 o1) (do s2 o2)) (do (do s3 o1) o2) /\
-                    eq (merge l (do s1 o) (do s2 o')) (do (do s3 o) o') /\ //***EXTRA***
-                    (forall e. eq_e (sel_e (merge (do l o') (do (do (do s1 o) o') o1) (do (do s2 o') o2)) e)
-                               (sel_e (do (do (do (do s3 o) o') o1) o2) e)))
-          (ensures eq (merge (do l o') (do (do (do s1 o) o') o1) (do (do s2 o') o2)) (do (do (do (do s3 o) o') o1) o2)) = ()
+let inter_right_base_2op_comm (l a b :concrete_st) (o1 o2 ob ol:op_t)
+  : Lemma (requires Either? (rc o2 o1) /\ get_rid o1 <> get_rid o2 /\ Fst_then_snd? (rc ob ol) /\ get_rid ob <> get_rid ol /\
+                    eq (merge l (do a o1) (do (do b ob) o2)) (do (merge l a (do (do b ob) o2)) o1) /\ //from ind_right_2op
+                    eq (merge (do l ol) (do (do a ol) o1) (do (do b ol) o2)) (do (merge (do l ol) (do a ol) (do (do b ol) o2)) o1))
+          (ensures eq (merge (do l ol) (do (do a ol) o1) (do (do (do b ob) ol) o2)) (do (merge (do l ol) (do a ol) (do (do (do b ob) ol) o2)) o1)) = ()
           
-//If we remove the last pre-condition and try to prove, we get assertion failure. (NOTE:eq_e is the equivalence relation of the ew flag)
-//So we have to do case splits in the proof (given in comments). But while proving one case we need to admit the other cases. 
-//It will be good if we can prove the lemma automatically (without case splits) and without the last pre-condition.
-(*let rc_intermediate_base_left_right' (l s1 s2 s3:concrete_st) (o o' o1' o1 o2:op_t) 
-  : Lemma (requires distinct_ops o o' /\ Fst_then_snd? (rc o o') /\  
-                    distinct_ops o1 o2 /\ Fst_then_snd? (rc o1 o2) /\
-                    distinct_ops o1' o' /\ Fst_then_snd? (rc o1' o') /\
-                    eq (merge (do l o') (do (do s1 o') o1) (do (do s2 o') o2)) (do (do (do s3 o') o1) o2) /\
-                    eq (merge l (do s1 o1) (do s2 o2)) (do (do s3 o1) o2) /\
-                    (forall e. eq_e (sel_e (merge (do l o') (do (do (do s1 o1') o') o1) (do (do (do s2 o) o') o2)) e)
-                               (sel_e (do (do (do (do (do s3 o1') o) o') o1) o2) e))) 
-        (ensures eq (merge (do l o') (do (do (do s1 o1') o') o1) (do (do (do s2 o) o') o2)) (do (do (do (do (do s3 o1') o) o') o1) o2)) = ()*)
-  (*if get_ele o2 = get_ele o' && get_rid o2 = get_rid o' then () //done
-  else if get_ele o2 = get_ele o' && get_rid o2 <> get_rid o' then () //done
-  else if get_ele o2 <> get_ele o' && get_rid o2 = get_rid o' then () //done
-  else () //done*)
+let inter_right_base_2op l a b o1 o2 ob ol = 
+  if Fst_then_snd? (rc o2 o1) then inter_right_base_2op_fts l a b o1 o2 ob ol
+  else inter_right_base_2op_comm l a b o1 o2 ob ol
+     
+let inter_left_base_2op l a b o1 o2 ob ol = ()
 
-let rc_inter_right' (l s1 s2 s3:concrete_st) (o1 o2 o o' o_n:op_t)
-  : Lemma (requires distinct_ops o1 o2 /\ Fst_then_snd? (rc o1 o2) /\  
-                    distinct_ops o o' /\ Fst_then_snd? (rc o o') /\
-                    get_rid o_n <> get_rid o' (*o_n,o' must be concurrent*) /\
-                    ((~ (commutes_with o_n o)) \/ Fst_then_snd? (rc o_n o')) /\
-                    eq (merge (do l o') (do (do s1 o') o1) (do (do (do s2 o) o') o2)) (do (do (do (do s3 o) o') o1) o2) /\
-                    (forall e. eq_e (sel_e (merge (do l o') (do (do s1 o') o1) (do (do (do (do s2 o_n) o) o') o2)) e)
-                               (sel_e (do (do (do (do (do s3 o_n) o) o') o1) o2) e)))
-          (ensures eq (merge (do l o') (do (do s1 o') o1) (do (do (do (do s2 o_n) o) o') o2)) (do (do (do (do (do s3 o_n) o) o') o1) o2)) = ()
-  (*assert (Add? (snd (snd o_n)) /\ get_ele o_n = get_ele o');
-  if get_ele o2 = get_ele o' && get_rid o2 = get_rid o' then () //done
-  else if get_ele o2 = get_ele o' && get_rid o2 <> get_rid o' then () //done
-  else if get_ele o2 <> get_ele o' && get_rid o2 = get_rid o' then () //done
-  else () //done*)
+let inter_right_2op_fts (l a b:concrete_st) (o1 o2 ob ol o:op_t) 
+  : Lemma (requires Fst_then_snd? (rc o2 o1) /\ get_rid o1 <> get_rid o2 /\ Fst_then_snd? (rc ob ol) /\ get_rid ob <> get_rid ol /\
+                    (~ (Either? (rc o ob)) \/ Fst_then_snd? (rc o ol)) /\
+                    eq (merge (do l ol) (do (do a ol) o1) (do (do (do b ob) ol) o2)) (do (merge (do l ol) (do a ol) (do (do (do b ob) ol) o2)) o1))
+          (ensures eq (merge (do l ol) (do (do a ol) o1) (do (do (do (do b o) ob) ol) o2)) (do (merge (do l ol) (do a ol) (do (do (do (do b o) ob) ol) o2)) o1)) = ()
 
-let rc_inter_left' (l s1 s2 s3:concrete_st) (o1 o2 o o':op_t) (o_n:op_t{~ (commutes_with o_n o)})
-  : Lemma (requires distinct_ops o1 o2 /\ Fst_then_snd? (rc o1 o2) /\  
-                    distinct_ops o o' /\ Fst_then_snd? (rc o o') /\
-                    get_rid o_n <> get_rid o' (*o_n,o' must be concurrent*) /\
-                    ((~ (commutes_with o_n o)) \/ Fst_then_snd? (rc o_n o')) /\
-                    eq (merge (do l o') (do (do (do s1 o) o') o1) (do (do s2 o') o2)) (do (do (do (do s3 o) o') o1) o2) /\
-                    (forall e. eq_e (sel_e (merge (do l o') (do (do (do (do s1 o_n) o) o') o1) (do (do s2 o') o2)) e)
-                              (sel_e (do (do (do (do (do s3 o_n) o) o') o1) o2) e)))
-      (ensures eq (merge (do l o') (do (do (do (do s1 o_n) o) o') o1) (do (do s2 o') o2)) (do (do (do (do (do s3 o_n) o) o') o1) o2)) = ()
-  (*assert (Add? (snd (snd o_n)) /\ get_ele o_n = get_ele o');
-  if get_ele o2 = get_ele o' && get_rid o2 = get_rid o' then () //done
-  else if get_ele o2 = get_ele o' && get_rid o2 <> get_rid o' then () //done
-  else if get_ele o2 <> get_ele o' && get_rid o2 = get_rid o' then () //done
-  else () //done*)
+let inter_right_2op_comm (l a b:concrete_st) (o1 o2 ob ol o:op_t) 
+  : Lemma (requires Either? (rc o2 o1) /\ get_rid o1 <> get_rid o2 /\ Fst_then_snd? (rc ob ol) /\ get_rid ob <> get_rid ol /\
+                    (~ (Either? (rc o ob)) \/ Fst_then_snd? (rc o ol)) /\
+                    get_rid o <> get_rid ol /\
+                    eq (merge (do l ol) (do (do a ol) o1) (do (do (do b ob) ol) o2)) (do (merge (do l ol) (do a ol) (do (do (do b ob) ol) o2)) o1))
+          (ensures eq (merge (do l ol) (do (do a ol) o1) (do (do (do (do b o) ob) ol) o2)) (do (merge (do l ol) (do a ol) (do (do (do (do b o) ob) ol) o2)) o1)) = ()
 
-let rc_inter_lca' (l s1 s2 s3:concrete_st) (o1 o2 o' o_n:op_t)
-  : Lemma (requires distinct_ops o1 o2 /\ Fst_then_snd? (rc o1 o2) /\ 
-                    (exists o. Fst_then_snd? (rc o o')) /\ (exists o. Fst_then_snd? (rc o o_n)) /\ 
-                    eq (merge (do l o_n) (do (do s1 o_n) o1) (do (do s2 o_n) o2)) (do (do (do s3 o_n) o1) o2) /\
-                    eq (merge (do l o') (do (do s1 o') o1) (do (do s2 o') o2)) (do (do (do s3 o') o1) o2) /\
-                    (forall e. eq_e (sel_e (merge (do (do l o_n) o') (do (do (do s1 o_n) o') o1) (do (do (do s2 o_n) o') o2)) e)
-                               (sel_e (do (do (do (do s3 o_n) o') o1) o2) e)))
-    (ensures eq (merge (do (do l o_n) o') (do (do (do s1 o_n) o') o1) (do (do (do s2 o_n) o') o2)) (do (do (do (do s3 o_n) o') o1) o2)) = ()
+let inter_right_2op l a b o1 o2 ob ol o = 
+  if Fst_then_snd? (rc o2 o1) then inter_right_2op_fts l a b o1 o2 ob ol o
+  else inter_right_2op_comm l a b o1 o2 ob ol o
 
-(*One op*)
-///////////////
-let one_op_ind_right' (l a b c:concrete_st) (o1 o1':op_t)
-   : Lemma (requires eq (merge l a (do b o1)) (do (merge l a b) o1) /\
-                     (forall e. eq_e (sel_e (merge l a (do (do b o1') o1)) e) (sel_e (do (merge l a (do b o1')) o1) e)))
-           (ensures eq (merge l a (do (do b o1') o1)) (do (merge l a (do b o1')) o1)) = ()
-           
-let one_op_ind_lca' (l:concrete_st) (o o1:op_t)
-  : Lemma (requires eq (merge l l (do l o1)) (do l o1) /\
-                    (forall e. eq_e (sel_e (merge (do l o) (do l o) (do (do l o) o1)) e) (sel_e (do (do l o) o1) e)))
-          (ensures eq (merge (do l o) (do l o) (do (do l o) o1)) (do (do l o) o1)) = ()
+let inter_left_2op l a b o1 o2 ob ol o = ()
 
-let one_op_base' (o1:op_t)
-  : Lemma (ensures eq (merge init_st init_st (do init_st o1)) (do init_st o1)) = ()
+let ind_right_2op l a b o1 o2 o2' = ()
 
-let one_op_inter_base_right' (l s1 s2 s3:concrete_st) (o o' o1:op_t) 
-  : Lemma (requires distinct_ops o o' /\ Fst_then_snd? (rc o o') /\
-                    eq (merge (do l o') (do s1 o') (do (do s2 o') o1)) (do (do s3 o') o1) /\
-                    eq (merge l s1 (do s2 o1)) (do s3 o1) /\
-                    eq (merge l (do s1 o') (do s2 o)) (do (do s3 o) o') /\ //***EXTRA***
-                    (forall e. eq_e (sel_e (merge (do l o') (do s1 o') (do (do (do s2 o) o') o1)) e) (sel_e (do (do (do s3 o) o') o1) e)))
-          (ensures eq (merge (do l o') (do s1 o') (do (do (do s2 o) o') o1)) (do (do (do s3 o) o') o1)) = ()
+let ind_left_2op l a b o1 o2 o1' = ()
 
-(*let intermediate_base_right_one_op_left' (l s1 s2 s3:concrete_st) (o o' o1:op_t) 
-  : Lemma (requires distinct_ops o o' /\ Fst_then_snd? (rc o o') /\ distinct_ops o' o1 /\
-                    eq (merge (do l o') (do (do s1 o') o1) (do s2 o')) (do (do s3 o') o1) /\
-                    (Fst_then_snd? (rc o o1) ==> eq (merge l (do s1 o1) (do s2 o)) (do (merge l s1 (do s2 o)) o1)) /\ //***EXTRA***       
-                    eq (merge l (do s1 o1) s2) (do s3 o1) /\
-                    eq (merge l (do s1 o') (do s2 o)) (do (do s3 o) o') /\ //***EXTRA***
-                    (forall e. eq_e (sel_e (merge (do l o') (do (do s1 o') o1) (do (do s2 o) o')) e) (sel_e (do (do (do s3 o) o') o1) e)))
-          (ensures eq (merge (do l o') (do (do s1 o') o1) (do (do s2 o) o')) (do (do (do s3 o) o') o1)) = ()*)
-  (*let lhs = (merge (do l o') (do (do s1 o') o1) (do (do s2 o) o')) in
-  let rhs = (do (do (do s3 o) o') o1) in
-  
-  if Add? (snd (snd o1)) && get_ele o1 = get_ele o' && get_rid o1 = get_rid o' then () //done
-  else if Add? (snd (snd o1)) && get_ele o1 = get_ele o' && get_rid o1 <> get_rid o' then 
-    (assume (fst (sel_id (sel_e (do s1 o') (get_ele o1)) (get_rid o1)) >= fst (sel_id (sel_e l (get_ele o1)) (get_rid o1))); //todo
-     assert (snd (sel_id (sel_e lhs (get_ele o1)) (get_rid o1)) = snd (sel_id (sel_e rhs (get_ele o1)) (get_rid o1)));
-     ())
-  else if Add? (snd (snd o1)) && get_ele o1 <> get_ele o' && get_rid o1 = get_rid o' then () //done
-  else if Add? (snd (snd o1)) && get_ele o1 <> get_ele o' && get_rid o1 <> get_rid o' then () //done
-  else if Rem? (snd (snd o1)) && get_ele o1 = get_ele o' then ()
-  else ()*)
+let base_1op o1 = ()
 
-let one_op_inter_base_left' (l s1 s2 s3:concrete_st) (o o' o1:op_t) 
-  : Lemma (requires distinct_ops o o' /\ Fst_then_snd? (rc o o') /\
-                    eq (merge (do l o') (do s1 o') (do (do s2 o') o1)) (do (do s3 o') o1) /\
-                    (Fst_then_snd? (rc o o1) ==> eq (merge l (do s1 o1) (do s2 o)) (do (merge l s1 (do s2 o)) o1)) /\ //***EXTRA***
-                    eq (merge l s1 (do s2 o1)) (do s3 o1) /\
-                    eq (merge l (do s1 o') (do s2 o)) (do (do s3 o) o') /\ //***EXTRA***
-                    eq (merge l (do (do s1 o) o') (do s2 o')) (do (do s3 o) o') /\ //***EXTRA***
-                    (forall e. eq_e (sel_e (merge (do l o') (do (do s1 o) o') (do (do s2 o') o1)) e)
-                               (sel_e (do (do (do s3 o) o') o1) e)))
-          (ensures eq (merge (do l o') (do (do s1 o) o') (do (do s2 o') o1)) (do (do (do s3 o) o') o1)) = ()
-  (*if Add? (snd (snd o1)) && get_ele o1 = get_ele o' && get_rid o1 = get_rid o' then () //done
-  else if Add? (snd (snd o1)) && get_ele o1 = get_ele o' && get_rid o1 <> get_rid o' then () //done
-  else if Add? (snd (snd o1)) && get_ele o1 <> get_ele o' && get_rid o1 = get_rid o' then () //done
-  else if Add? (snd (snd o1)) && get_ele o1 <> get_ele o' && get_rid o1 <> get_rid o' then () //done
-  else if Rem? (snd (snd o1)) && get_ele o1 = get_ele o' then () //done
-  else () //done*)
+let ind_lca_1op l o1 ol = ()
 
-(*let intermediate_base_left_right_one_op' (l s1 s2 s3:concrete_st) (o o' o1' o1:op_t) 
-  : Lemma (requires distinct_ops o o' /\ Fst_then_snd? (rc o o') /\
-                    distinct_ops o1' o' /\ Fst_then_snd? (rc o1' o') /\
-                    eq (merge (do l o') (do s1 o') (do (do s2 o') o1)) (do (do s3 o') o1) /\
-                    eq (merge (do l o') (do (do s1 o1') o') (do (do s2 o') o1)) (do (do (do s3 o1') o') o1) /\ //EXTRA
-                    eq (merge l s1 (do s2 o1)) (do s3 o1) /\
-                    (forall e. eq_e (sel_e (merge (do l o') (do (do s1 o1') o') (do (do (do s2 o) o') o1)) e)
-                               (sel_e (do (do (do (do s3 o1') o) o') o1) e)))
-          (ensures eq (merge (do l o') (do (do s1 o1') o') (do (do (do s2 o) o') o1)) (do (do (do (do s3 o1') o) o') o1)) = ()*)
-  (*assert (Either? (rc o o1'));
-  let lhs = (merge (do l o') (do (do s1 o1') o') (do (do (do s2 o) o') o1)) in
-  let rhs = (do (do (do (do s3 o1') o) o') o1) in
-  if Add? (snd (snd o1)) && get_ele o1 = get_ele o' && get_rid o1 = get_rid o' then () //done
-  else if Add? (snd (snd o1)) && get_ele o1 = get_ele o' && get_rid o1 <> get_rid o' then 
-    (assert (forall ele rid. fst (sel_id (sel_e lhs ele) rid) = fst (sel_id (sel_e rhs ele) rid)); //done
-     assert (forall ele rid. snd (sel_id (sel_e lhs ele) rid) = snd (sel_id (sel_e rhs ele) rid)); //done
-     ())
-  else if Add? (snd (snd o1)) && get_ele o1 <> get_ele o' && get_rid o1 = get_rid o' then () // done
-  else if Add? (snd (snd o1)) && get_ele o1 <> get_ele o' && get_rid o1 <> get_rid o' then () // done
-  else if Rem? (snd (snd o1)) && get_ele o1 = get_ele o' then () // done
-  else () // done*)
+let inter_right_base_1op l a b o1 ob ol = ()
+     
+let inter_left_base_1op l a b o1 ob ol = ()
 
-let one_op_inter_left' (l s1 s2 s3:concrete_st) (o1 o o':op_t) (o_n:op_t{~ (commutes_with o_n o)})
-  : Lemma (requires distinct_ops o o' /\ Fst_then_snd? (rc o o') /\
-                    get_rid o_n <> get_rid o' (*o_n,o' must be concurrent*) /\
-                    eq (merge (do l o') (do (do s1 o) o') (do (do s2 o') o1)) (do (do (do s3 o) o') o1) /\
-                    (forall e. eq_e (sel_e (merge (do l o') (do (do (do s1 o_n) o) o') (do (do s2 o') o1)) e)
-                               (sel_e (do (do (do (do s3 o_n) o) o') o1) e)))
-      (ensures eq (merge (do l o') (do (do (do s1 o_n) o) o') (do (do s2 o') o1)) (do (do (do (do s3 o_n) o) o') o1)) = ()
-  (*assert (Add? (snd (snd o_n)) && get_ele o_n = get_ele o');
-  if Add? (snd (snd o1)) && get_ele o1 = get_ele o' && get_rid o1 = get_rid o' then () //done
-  else if Add? (snd (snd o1)) && get_ele o1 = get_ele o' && get_rid o1 <> get_rid o' then () //done
-  else if Add? (snd (snd o1)) && get_ele o1 <> get_ele o' && get_rid o1 = get_rid o' then () //done
-  else if Add? (snd (snd o1)) && get_ele o1 <> get_ele o' && get_rid o1 <> get_rid o' then () //done
-  else if Rem? (snd (snd o1)) && get_ele o1 = get_ele o' then () //done
-  else () //done*)
+let inter_right_1op l a b o1 ob ol o = ()
 
-// In general, the events o',o_n, below should be such that these exists o, (rc o o')
-let one_op_inter_lca' (l s1 s2 s3:concrete_st) (o1 o' o_n:op_t)
-  : Lemma (requires (exists o. Fst_then_snd? (rc o o')) /\ (exists o. Fst_then_snd? (rc o o_n)) /\ 
-                    eq (merge (do l o_n) (do s1 o_n) (do (do s2 o_n) o1)) (do (do s3 o_n) o1) /\
-                    eq (merge (do l o') (do s1 o') (do (do s2 o') o1)) (do (do s3 o') o1) /\
-                    (forall e. eq_e (sel_e (merge (do (do l o_n) o') (do (do s1 o_n) o') (do (do (do s2 o_n) o') o1)) e)
-                               (sel_e (do (do (do s3 o_n) o') o1) e)))
-          (ensures eq (merge (do (do l o_n) o') (do (do s1 o_n) o') (do (do (do s2 o_n) o') o1)) (do (do (do s3 o_n) o') o1)) = ()
+let inter_left_1op (l a b:concrete_st) (o1 ob ol o:op_t) 
+  : Lemma (requires Fst_then_snd? (rc ob ol) /\ get_rid ob <> get_rid ol /\
+                    (~ (Either? (rc o ob)) \/ Fst_then_snd? (rc o ol)) /\
+                    get_rid o <> get_rid ol /\ //from app.fsti
+                    eq (merge (do l ol) (do (do (do a ob) ol) o1) (do b ol)) (do (merge (do l ol) (do (do a ob) ol) (do b ol)) o1))
+          (ensures eq (merge (do l ol) (do (do (do (do a o) ob) ol) o1) (do b ol)) (do (merge (do l ol) (do (do (do a o) ob) ol) (do b ol)) o1)) = ()
+ 
+let ind_left_1op l a b o1 o1' ol = ()
 
-(*Zero op *)
-///////////////
-let zero_op_inter_base_right' (l s1 s2 s3:concrete_st) (o o':op_t) 
-  : Lemma (requires distinct_ops o o' /\ Fst_then_snd? (rc o o') /\
-                    eq (merge (do l o') (do s1 o') (do s2 o')) (do s3 o') /\
-                    eq (merge l s1 s2) s3 /\
-                    eq (merge l (do s1 o') (do s2 o)) (do (do s3 o) o') /\ //***EXTRA***
-                    (forall e. eq_e (sel_e (merge (do l o') (do s1 o') (do (do s2 o) o')) e) (sel_e (do (do s3 o) o') e)))
-          (ensures eq (merge (do l o') (do s1 o') (do (do s2 o) o')) (do (do s3 o) o')) = ()
+let ind_right_1op l a b o2 o2' ol = ()
 
-let zero_op_inter_base_left' (l s1 s2 s3:concrete_st) (o o' o1':op_t) 
-  : Lemma (requires distinct_ops o o' /\ Fst_then_snd? (rc o o') /\  
-                    distinct_ops o1' o' /\ Fst_then_snd? (rc o1' o') /\
-                    eq (merge (do l o') (do s1 o') (do s2 o')) (do s3 o') /\
-                    eq (merge l s1 s2) s3 /\
-                    (forall e. eq_e (sel_e (merge (do l o') (do (do s1 o1') o') (do (do s2 o) o')) e) (sel_e  (do (do (do s3 o1') o) o') e)))
-          (ensures eq (merge (do l o') (do (do s1 o1') o') (do (do s2 o) o')) (do (do (do s3 o1') o) o')) = ()
-          
-(*let intermediate_base_left_right_zero_op' (l s1 s2 s3:concrete_st) (o o' o1':op_t) 
-  : Lemma (requires distinct_ops o o' /\ Fst_then_snd? (rc o o') /\  
-                    distinct_ops o1' o' /\ Fst_then_snd? (rc o1' o') /\
-                    eq (merge (do l o') (do s1 o') (do s2 o')) (do s3 o') /\
-                    eq (merge l s1 s2) s3 /\
-                    (forall e. eq_e (sel_e (merge (do l o') (do (do s1 o1') o') (do (do s2 o) o')) e)
-                               (sel_e (do (do (do s3 o1') o) o') e)))
-          (ensures eq (merge (do l o') (do (do s1 o1') o') (do (do s2 o) o')) (do (do (do s3 o1') o) o')) = ()*)
-
-let zero_op_inter_right' (l s1 s2 s3:concrete_st) (o o':op_t) (o_n:op_t{~ (commutes_with o_n o)})
-  : Lemma (requires distinct_ops o o' /\ Fst_then_snd? (rc o o') /\
-                    get_rid o_n <> get_rid o' (*o_n,o' must be concurrent*) /\
-                    eq (merge (do l o') (do s1 o') (do (do s2 o) o')) (do (do s3 o) o') /\
-                    (forall e. eq_e (sel_e (merge (do l o') (do s1 o') (do (do (do s2 o_n) o) o')) e) (sel_e (do (do (do s3 o_n) o) o') e)))
-      (ensures eq (merge (do l o') (do s1 o') (do (do (do s2 o_n) o) o')) (do (do (do s3 o_n) o) o')) = ()
-  (*assert (Fst_then_snd? (rc o o_n) && get_ele o = get_ele o_n);
-  assert (Either? (rc o' o_n));
-  if get_ele o_n = get_ele o' then () //done
-  else ()*)
-
-let zero_op_inter_left' (l s1 s2 s3:concrete_st) (o o':op_t) (o_n:op_t{~ (commutes_with o_n o)})
-  : Lemma (requires distinct_ops o o' /\ Fst_then_snd? (rc o o') /\
-                    get_rid o_n <> get_rid o' (*o_n,o' must be concurrent*) /\
-                    eq (merge (do l o') (do (do s1 o) o') (do s2 o')) (do (do s3 o) o') /\
-                    (forall e. eq_e (sel_e (merge (do l o') (do (do (do s1 o_n) o) o') (do s2 o')) e) (sel_e (do (do (do s3 o_n) o) o') e)))
-      (ensures eq (merge (do l o') (do (do (do s1 o_n) o) o') (do s2 o')) (do (do (do s3 o_n) o) o')) = ()
-  (*assert (Fst_then_snd? (rc o o_n) && get_ele o = get_ele o_n);
-  assert (Either? (rc o' o_n));
-  if get_ele o_n = get_ele o' then () //done
-  else ()*)
-
-// In general, the event "o" below should be such that these exists o', (rc o' o)
-let zero_op_inter_lca_v1' (l s1 s2 s3:concrete_st) (o:op_t)
-  : Lemma (requires (exists o'. Fst_then_snd? (rc o' o)) /\ eq (merge l s1 s2) s3)
-          (ensures eq (merge (do l o) (do s1 o) (do s2 o)) (do s3 o) ) = ()
-
-// In general, the events o',o_n, below should be such that these exists o, (rc o o')
-let zero_op_inter_lca_v2' (l s1 s2 s3:concrete_st) (o' o_n:op_t)
-  : Lemma (requires (exists o. Fst_then_snd? (rc o o')) /\ (exists o. Fst_then_snd? (rc o o_n)) /\ 
-                    eq (merge (do l o_n) (do s1 o_n) (do s2 o_n)) (do s3 o_n)  /\
-                    eq (merge (do l o') (do s1 o') (do s2 o')) (do s3 o') /\
-                    (forall e. eq_e (sel_e (merge (do (do l o_n) o') (do (do s1 o_n) o') (do (do s2 o_n) o')) e)
-                               (sel_e (do (do s3 o_n) o') e)))
-          (ensures eq (merge (do (do l o_n) o') (do (do s1 o_n) o') (do (do s2 o_n) o')) (do (do s3 o_n) o')) = ()
-
-(* 2 op Comm  *)
-///////////////////
-
-let comm_ind_right' (l a b c:concrete_st) (o1 o2' o2:op_t)
-  : Lemma (requires distinct_ops o1 o2 /\ Either? (rc o1 o2) /\ distinct_ops o2' o1 /\
-                    eq (merge l (do a o1) (do b o2)) (do (do (merge l a b) o2) o1) /\
-                    (Fst_then_snd? (rc o2' o1) ==> (eq (merge l (do a o1) (do b o2')) (do (merge l a (do b o2')) o1))) /\
-                    ~ (exists o3 a'. eq (do a o1) (do a' o3) /\ distinct_ops o2 o3 /\ Fst_then_snd? (rc o2 o3)) /\
-                    ~ (Fst_then_snd? (rc o1 o2')) /\
-                    ~ (exists o3 b'. eq (do (do b o2') o2) (do b' o3) /\ distinct_ops o1 o3 /\ Fst_then_snd? (rc o1 o3)) /\
-                    ~ (exists o3 b'. eq (do b o2) (do b' o3) /\ distinct_ops o1 o3 /\ Fst_then_snd? (rc o1 o3)) /\
-                    (forall e. eq_e (sel_e (merge l (do a o1) (do (do b o2') o2)) e) (sel_e (do (do (merge l a (do b o2')) o2) o1) e)))      
-          (ensures eq (merge l (do a o1) (do (do b o2') o2)) (do (do (merge l a (do b o2')) o2) o1)) = ()
-  (*if Add? (snd (snd o1)) && Add? (snd (snd o2)) && get_ele o1 = get_ele o2 then () //done
-  else if Add? (snd (snd o1)) && Add? (snd (snd o2)) && get_ele o1 <> get_ele o2 && Add? (snd (snd o2')) then () //done
-  else if Add? (snd (snd o1)) && Add? (snd (snd o2)) && get_ele o1 <> get_ele o2 && Rem? (snd (snd o2')) then () //done
-  else if Add? (snd (snd o1)) && Rem? (snd (snd o2)) then () //done
-  else if Rem? (snd (snd o1)) && Add? (snd (snd o2)) then () //done
-  else ()*)
-
-let comm_ind_left' (l a b c:concrete_st) (o1 o2' o2:op_t)
-  : Lemma (requires distinct_ops o1 o2 /\ Either? (rc o1 o2) /\ distinct_ops o2' o2 /\
-                    eq (merge l (do a o1) (do b o2)) (do (do (merge l a b) o2) o1) /\
-                    (Fst_then_snd? (rc o2' o2) ==> (eq (merge l (do a o2') (do b o2)) (do (merge l (do a o2') b) o2))) /\
-                    ~ (exists o3 a'. eq (do a o1) (do a' o3) /\ distinct_ops o2 o3 /\ Fst_then_snd? (rc o2 o3)) /\
-                    ~ (Fst_then_snd? (rc o2 o2')) /\
-                    ~ (exists o3 b'. eq (do (do b o2') o2) (do b' o3) /\ distinct_ops o1 o3 /\ Fst_then_snd? (rc o1 o3)) /\
-                    ~ (exists o3 b'. eq (do b o2) (do b' o3) /\ distinct_ops o1 o3 /\ Fst_then_snd? (rc o1 o3)) /\
-                    (forall e. eq_e (sel_e (merge l (do (do a o2') o1) (do b o2)) e) (sel_e (do (do (merge l (do a o2') b) o2) o1) e)))      
-          (ensures eq (merge l (do (do a o2') o1) (do b o2)) (do (do (merge l (do a o2') b) o2) o1)) = ()
-  (*if Add? (snd (snd o1)) && Add? (snd (snd o2)) && get_ele o1 = get_ele o2 then () //done
-  else if Add? (snd (snd o1)) && Add? (snd (snd o2)) && get_ele o1 <> get_ele o2 && Add? (snd (snd o2')) then () //done
-  else if Add? (snd (snd o1)) && Add? (snd (snd o2)) && get_ele o1 <> get_ele o2 && Rem? (snd (snd o2')) then () //done
-  else if Add? (snd (snd o1)) && Rem? (snd (snd o2)) then () //done
-  else if Rem? (snd (snd o1)) && Add? (snd (snd o2)) then () //done
-  else ()*)
-
-let comm_ind_lca' (l:concrete_st) (o o1 o2:op_t)
-  : Lemma (requires distinct_ops o1 o2 /\ Either? (rc o1 o2) /\ distinct_ops o o1 /\ distinct_ops o o2 /\
-                    eq (merge l (do l o1) (do l o2)) (do (do l o2) o1))
-          (ensures eq (merge (do l o) (do (do l o) o1) (do (do l o) o2)) (do (do (do l o) o2) o1)) = ()
-
-let comm_base' (o1 o2:op_t)
-  : Lemma (requires distinct_ops o1 o2 /\ Either? (rc o1 o2))
-          (ensures eq (merge init_st (do init_st o1) (do init_st o2)) (do (do init_st o1) o2)) = ()
-
-let comm_inter_base_right' (l s1 s2 s3:concrete_st) (o o' o1 o2:op_t) 
-  : Lemma (requires distinct_ops o o' /\ Fst_then_snd? (rc o o') /\ 
-                    distinct_ops o1 o2 /\ Either? (rc o1 o2) /\
-                    distinct_ops o' o1 /\ distinct_ops o' o2 /\
-                    eq (merge l (do s1 o1) (do (do s2 o) o2)) (do (do (merge l s1 (do s2 o)) o1) o2) /\ //comes from comm_ind_right
-                    eq (merge (do l o') (do (do s1 o') o1) (do (do s2 o') o2)) (do (do (do s3 o') o1) o2) /\ 
-                    eq (merge (do l o') (do s1 o') (do (do s2 o) o')) (do (do s3 o) o') /\ //comes from intermediate_base_zero_op
-                    eq (merge l (do s1 o1) (do s2 o2)) (do (do s3 o1) o2) /\
-                    (forall e. eq_e (sel_e (merge (do l o') (do (do s1 o') o1) (do (do (do s2 o) o') o2)) e)
-                               (sel_e (do (do (do (do s3 o) o') o1) o2) e)))
-          (ensures eq (merge (do l o') (do (do s1 o') o1) (do (do (do s2 o) o') o2)) (do (do (do (do s3 o) o') o1) o2)) = ()
-  (*if Rem? (snd (snd o1)) && Rem? (snd (snd o2)) then admit() //done
-  else if Add? (snd (snd o1)) && Rem? (snd (snd o2)) && get_ele o1 = get_ele o' then admit() //done
-  else if Add? (snd (snd o1)) && Rem? (snd (snd o2)) && get_ele o1 <> get_ele o' then admit() //done
-  else if Rem? (snd (snd o1)) && Add? (snd (snd o2)) && get_ele o2 = get_ele o' then admit() //done
-  else if Rem? (snd (snd o1)) && Add? (snd (snd o2)) && get_ele o2 <> get_ele o' then admit() //done
-  
-  else if get_ele o1 = get_ele o' && get_ele o2 = get_ele o' && get_rid o1 = get_rid o' && get_rid o2 = get_rid o' then admit() // done
-  else if get_ele o1 = get_ele o' && get_ele o2 = get_ele o' && get_rid o1 = get_rid o' && get_rid o2 <> get_rid o' then admit() // done
-  else if get_ele o1 = get_ele o' && get_ele o2 = get_ele o' && get_rid o1 <> get_rid o' && get_rid o2 = get_rid o' then admit() // done
-  else if get_ele o1 = get_ele o' && get_ele o2 = get_ele o' && get_rid o1 <> get_rid o' && get_rid o2 <> get_rid o' then admit() // not done
-
-  else if get_ele o1 = get_ele o' && get_ele o2 <> get_ele o' && get_rid o1 = get_rid o' && get_rid o2 = get_rid o' then admit() // done
-  else if get_ele o1 = get_ele o' && get_ele o2 <> get_ele o' && get_rid o1 = get_rid o' && get_rid o2 <> get_rid o' then admit() // done
-  else if get_ele o1 = get_ele o' && get_ele o2 <> get_ele o' && get_rid o1 <> get_rid o' && get_rid o2 = get_rid o' then admit() // done
-  else if get_ele o1 = get_ele o' && get_ele o2 <> get_ele o' && get_rid o1 <> get_rid o' && get_rid o2 <> get_rid o' then admit() // not done
-  
-  else admit() //not done*)
-
-(*let comm_intermediate_base_left_right' (l s1 s2 s3:concrete_st) (o o' o1' o1 o2:op_t) 
-  : Lemma (requires distinct_ops o o' /\ Fst_then_snd? (rc o o') /\ 
-                    distinct_ops o1 o2 /\ Either? (rc o1 o2) /\
-                    distinct_ops o1' o' /\ Fst_then_snd? (rc o1' o') /\
-                    distinct_ops o' o1 /\ distinct_ops o' o2 /\
-                    eq (merge (do l o') (do (do s1 o') o1) (do (do s2 o') o2)) (do (do (do s3 o') o1) o2) /\
-                    eq (merge l (do s1 o1) (do s2 o2)) (do (do s3 o1) o2) /\
-                    eq (merge l (do (do s1 o1') o1) (do (do s2 o) o2)) (do (do (merge l (do s1 o1') (do s2 o)) o1) o2) /\ //comes from comm_ind_right
-                    eq (merge (do l o') (do s1 o') (do (do s2 o) o')) (do (do s3 o) o') /\ //comes from intermediate_base_zero_op
-                    (forall e. eq_e (sel_e (merge (do l o') (do (do (do s1 o1') o') o1) (do (do (do s2 o) o') o2)) e)
-                               (sel_e (do (do (do (do (do s3 o1') o) o') o1) o2) e)))
-          (ensures eq (merge (do l o') (do (do (do s1 o1') o') o1) (do (do (do s2 o) o') o2)) (do (do (do (do (do s3 o1') o) o') o1) o2)) = ()*)
-
-let comm_inter_base_left' (l s1 s2 s3:concrete_st) (o o' o1 o2:op_t) 
-  : Lemma (requires distinct_ops o o' /\ Fst_then_snd? (rc o o') /\ 
-                    distinct_ops o1 o2 /\ Either? (rc o1 o2) /\
-                    distinct_ops o' o1 /\ distinct_ops o' o2 /\
-                    eq (merge l (do (do s1 o) o1) (do s2 o2)) (do (do (merge l (do s1 o) s2) o1) o2) /\ //comes from comm_ind_left
-                    eq (merge (do l o') (do (do s1 o') o1) (do (do s2 o') o2)) (do (do (do s3 o') o1) o2) /\ 
-                    eq (merge (do l o') (do (do s1 o) o') (do s2 o')) (do (do s3 o) o') /\ //comes from intermediate_base_zero_op
-                    eq (merge l (do s1 o1) (do s2 o2)) (do (do s3 o1) o2) /\
-                    (forall e. eq_e (sel_e (merge (do l o') (do (do (do s1 o) o') o1) (do (do s2 o') o2)) e) (sel_e (do (do (do (do s3 o) o') o1) o2) e)))
-          (ensures eq (merge (do l o') (do (do (do s1 o) o') o1) (do (do s2 o') o2)) (do (do (do (do s3 o) o') o1) o2)) = ()
-          
-let comm_inter_right' (l s1 s2 s3:concrete_st) (o1 o2 o o':op_t) (o_n:op_t{~ (commutes_with o_n o)})
-  : Lemma (requires distinct_ops o1 o2 /\ Either? (rc o1 o2) /\  
-                    distinct_ops o o' /\ Fst_then_snd? (rc o o') /\
-                    get_rid o_n <> get_rid o' (*o_n,o' must be concurrent*) /\
-                    distinct_ops o_n o' /\ Either? (rc o_n o') /\ 
-                    eq (merge (do l o') (do (do s1 o') o1) (do (do (do s2 o) o') o2)) (do (do (do (do s3 o) o') o1) o2) /\
-                    (forall e. eq_e (sel_e (merge (do l o') (do (do s1 o') o1) (do (do (do (do s2 o_n) o) o') o2)) e)
-                               (sel_e (do (do (do (do (do s3 o_n) o) o') o1) o2) e)))
-      (ensures eq (merge (do l o') (do (do s1 o') o1) (do (do (do (do s2 o_n) o) o') o2)) (do (do (do (do (do s3 o_n) o) o') o1) o2)) = ()
-  (*assume (Either? (rc o_n o') /\ Fst_then_snd? (rc o o') /\ get_ele o = get_ele o');
-  let lhs = (merge (do l o') (do (do s1 o') o1) (do (do (do (do s2 o_n) o) o') o2)) in
-  let rhs = (do (do (do (do (do s3 o_n) o) o') o1) o2) in
-  assume (forall ele. M.contains lhs ele = M.contains rhs ele);
-  assume (forall ele. M.contains lhs ele ==> (forall rid. M.contains (sel_e lhs ele) rid = M.contains (sel_e rhs ele) rid));
-  admit()*)
-
-let comm_inter_left' (l s1 s2 s3:concrete_st) (o1 o2 o o':op_t) (o_n:op_t{~ (commutes_with o_n o)})
-  : Lemma (requires distinct_ops o1 o2 /\ Either? (rc o1 o2) /\  
-                    distinct_ops o o' /\ Fst_then_snd? (rc o o') /\
-                    get_rid o_n <> get_rid o' (*o_n,o' must be concurrent*) /\
-                    distinct_ops o_n o' /\ Either? (rc o_n o') /\ 
-                    eq (merge (do l o') (do (do (do s1 o) o') o1) (do (do s2 o') o2)) (do (do (do (do s3 o) o') o1) o2) /\
-                    (forall e. eq_e (sel_e (merge (do l o') (do (do (do (do s1 o_n) o) o') o1) (do (do s2 o') o2)) e)
-                               (sel_e (do (do (do (do (do s3 o_n) o) o') o1) o2) e)))
-          (ensures eq (merge (do l o') (do (do (do (do s1 o_n) o) o') o1) (do (do s2 o') o2)) (do (do (do (do (do s3 o_n) o) o') o1) o2)) = ()
-
-let comm_inter_lca' (l s1 s2 s3:concrete_st) (o1 o2 o:op_t)
-  : Lemma (requires distinct_ops o1 o2 /\ Either? (rc o1 o2) /\ distinct_ops o1 o /\ distinct_ops o o2 /\
-                    (exists o'. Fst_then_snd? (rc o' o)) /\
-                    eq (merge l (do s1 o1) (do s2 o2)) (do (do s3 o1) o2) /\
-                    (forall e. eq_e (sel_e (merge (do l o) (do (do s1 o) o1) (do (do s2 o) o2)) e) (sel_e (do (do (do s3 o) o1) o2) e)))
-          (ensures eq (merge (do l o) (do (do s1 o) o1) (do (do s2 o) o2)) (do (do (do s3 o) o1) o2)) = ()
-  (*let lhs = (merge (do l o) (do (do s1 o) o1) (do (do s2 o) o2)) in
-  let rhs = (do (do (do s3 o) o1) o2) in
-  assume (forall ele. M.contains lhs ele = M.contains rhs ele);
-  assume (forall ele. M.contains lhs ele ==> (forall rid. M.contains (sel_e lhs ele) rid = M.contains (sel_e rhs ele) rid));
-  assume (forall ele rid. (ele <> get_ele o /\ rid <> get_rid o) ==> ( (sel_id (sel_e lhs ele) rid) =  (sel_id (sel_e rhs ele) rid)));
-  assume (forall ele rid. (ele <> get_ele o /\ rid = get_rid o) ==> (fst (sel_id (sel_e lhs ele) rid) = fst (sel_id (sel_e rhs ele) rid)));
-  assert (forall ele rid. (ele = get_ele o /\ rid <> get_rid o) ==> (fst (sel_id (sel_e lhs ele) rid) = fst (sel_id (sel_e rhs ele) rid)));
-  admit()*)
-
-////////////////////////////////////////////////////////////////
-//// Sequential implementation //////
-
-// the concrete state 
-let concrete_st_s' = S.t nat
-
-// init state 
-let init_st_s' = S.empty
-
-// apply an operation to a state 
-let do_s' (st_s:concrete_st_s') (o:op_t) : concrete_st_s' =
-  match o with
-  |(ts, (rid, Add e)) -> S.add e st_s
-  |(_, (rid, Rem e)) -> S.filter st_s (fun ele -> ele <> e)
-
-let mem_ele (ele:nat) (s:concrete_st) : prop =
-  exists rid. M.contains (sel_e s ele) rid /\ snd (sel_id (sel_e s ele) rid) = true
-  
-// equivalence relation between the concrete states of sequential type and MRDT
-let eq_sm' (st_s:concrete_st_s') (st:concrete_st) =
-  (forall e. S.mem e st_s <==> mem_ele e st)
-
-// initial states are equivalent
-let initial_eq' (_:unit)
-  : Lemma (ensures eq_sm' init_st_s' init_st) = ()
-
-// equivalence between states of sequential type and MRDT at every operation
-let do_eq' (st_s:concrete_st_s') (st:concrete_st) (op:op_t)   
-  : Lemma (requires eq_sm' st_s st)
-          (ensures eq_sm' (do_s' st_s op) (do st op)) =
-  if Add? (snd (snd op)) then 
-    (if S.mem (get_ele op) st_s then () else ())
-  else ()
-
-////////////////////////////////////////////////////////////////
+let lem_0op l a b ol = ()
