mrdts-new/RGA-no-pre/App_new.fst
@@ -1,0 +1,128 @@
+module App_new
+
+module S = Set_extended
+
+#set-options "--query_stats"
+
+// the concrete state type
+type concrete_st = S.t (nat & (nat & nat)) & S.t nat //fst:(ts,after_id,ele), snd:tombstone set
+
+// init state
+let init_st = (S.empty, S.empty)
+
+// equivalence between 2 concrete states
+let eq (a b:concrete_st) = 
+  S.equal (fst a) (fst b) /\
+  S.equal (snd a) (snd b)
+
+let symmetric (a b:concrete_st) 
+  : Lemma (requires eq a b)
+          (ensures eq b a) = ()
+
+let transitive (a b c:concrete_st)
+  : Lemma (requires eq a b /\ eq b c)
+          (ensures eq a c) = ()
+
+let eq_is_equiv (a b:concrete_st)
+  : Lemma (requires a == b)
+          (ensures eq a b) = ()
+
+// operation type
+type app_op_t:eqtype = 
+  |Add_after : after_id:nat -> ele:nat -> app_op_t //inserts ele after after_id
+  |Remove : id:pos -> app_op_t //removes the element with identifier id
+
+let get_ele (op:op_t{Add_after? (snd (snd op))}) : nat =
+  let (_, (_, Add_after _ ele)) = op in ele
+
+let get_after_id (op:op_t{Add_after? (snd (snd op))}) : nat =
+  let (_, (_, Add_after id _)) = op in id
+
+let get_rem_id (op:op_t{Remove? (snd (snd op))}) : pos =
+  let (_, (_, Remove id)) = op in id
+
+let id_ele (s:concrete_st) (id ele:nat) =
+  exists e. S.mem e (fst s) /\ fst e = id /\ snd (snd e) = ele /\ not (S.mem id (snd s))
+
+let mem_id_s (id:nat) (s:S.t (nat & (nat & nat))) =
+  exists e. S.mem e s /\ fst e = id
+  
+// apply an operation to a state
+let do (s:concrete_st) (o:op_t) : concrete_st =
+  match o with
+  |(ts, (_, Add_after after_id ele)) -> (S.add (ts, (after_id, ele)) (fst s), snd s)
+  |(_, (_, Remove id)) -> (fst s, S.add id (snd s))
+
+//conflict resolution
+let rc (o1 o2:op_t) = Either
+
+// concrete merge operation
+let merge (l a b:concrete_st) : concrete_st =
+   (S.union (fst l) (S.union (fst a) (fst b)),   
+    S.union (snd l) (S.union (snd a) (snd b)))
+   
+/////////////////////////////////////////////////////////////////////////////
+
+#push-options "--z3rlimit 100 --max_ifuel 3"
+let rc_non_comm (o1 o2:op_t)
+  : Lemma (requires distinct_ops o1 o2)
+          (ensures Either? (rc o1 o2) <==> commutes_with o1 o2) = ()
+  
+let no_rc_chain (o1 o2 o3:op_t)
+  : Lemma (requires distinct_ops o1 o2 /\ distinct_ops o2 o3)
+          (ensures ~ (Fst_then_snd? (rc o1 o2) /\ Fst_then_snd? (rc o2 o3))) = ()
+
+let cond_comm_base (s:concrete_st) (o1 o2 o3:op_t) 
+  : Lemma (requires distinct_ops o1 o2 /\ distinct_ops o2 o3 /\ distinct_ops o1 o3 /\
+                    Fst_then_snd? (rc o1 o2) /\ ~ (Either? (rc o2 o3)))
+          (ensures eq (do (do (do s o1) o2) o3) (do (do (do s o2) o1) o3)) = ()
+
+let cond_comm_ind (s:concrete_st) (o1 o2 o3 o:op_t) (l:seq op_t)
+  : Lemma (requires distinct_ops o1 o2 /\ distinct_ops o1 o3 /\ distinct_ops o2 o3 /\ 
+                    Fst_then_snd? (rc o1 o2) /\ ~ (Either? (rc o2 o3)) /\
+                    eq (do (apply_log (do (do s o1) o2) l) o3) (do (apply_log (do (do s o2) o1) l) o3))
+          (ensures eq (do (do (apply_log (do (do s o1) o2) l) o) o3) (do (do (apply_log (do (do s o2) o1) l) o) o3)) = ()
+ 
+/////////////////////////////////////////////////////////////////////////////
+// Merge commutativity
+let merge_comm (l a b:concrete_st)
+   : Lemma (ensures (eq (merge l a b) (merge l b a))) = ()
+
+// Merge idempotence
+let merge_idem (s:concrete_st)
+   : Lemma (ensures eq (merge s s s) s) = ()
+
+#set-options "--z3rlimit 300 --ifuel 3"
+let base_2op o1 o2 = ()
+
+let ind_lca_2op l o1 o2 ol = ()
+
+let inter_right_base_2op l a b o1 o2 ob ol = ()
+     
+let inter_left_base_2op l a b o1 o2 ob ol = ()
+
+let inter_right_2op l a b o1 o2 ob ol o = ()
+
+let inter_left_2op l a b o1 o2 ob ol o = ()
+
+let ind_right_2op l a b o1 o2 o2' = ()
+
+let ind_left_2op l a b o1 o2 o1' = ()
+
+let base_1op o1 = ()
+
+let ind_lca_1op l o1 ol = ()
+
+let inter_right_base_1op l a b o1 ob ol = ()
+     
+let inter_left_base_1op l a b o1 ob ol = ()
+   
+let inter_right_1op l a b o1 ob ol o = ()
+
+let inter_left_1op l a b o1 ob ol o = ()
+
+let ind_left_1op l a b o1 o1' ol = ()
+
+let ind_right_1op l a b o2 o2' ol = ()
+
+let lem_0op l a b ol = ()
