mrdts-new/Remove-wins_set/App_new.fst
@@ -1,0 +1,135 @@
+module App_new
+
+module S = Set_extended
+
+#set-options "--query_stats"
+
+// the concrete state type
+type concrete_st = s:S.t (nat * nat){forall e. S.mem e s ==> ((snd e = 1) \/ (snd e = 2))} //(nat & nat)
+
+// init state
+let init_st : concrete_st = S.add (0,1) (S.add (0,2) S.empty)
+
+// equivalence between 2 concrete states
+let eq (a b:concrete_st) =
+  forall e. S.mem e a = S.mem e b
+//S.equal a b
+
+let symmetric (a b:concrete_st) 
+  : Lemma (requires eq a b)
+          (ensures eq b a) = ()
+
+let transitive (a b c:concrete_st)
+  : Lemma (requires eq a b /\ eq b c)
+          (ensures eq a c) = ()
+
+let eq_is_equiv (a b:concrete_st)
+  : Lemma (requires a == b)
+          (ensures eq a b) = ()
+
+// operation type
+type app_op_t:eqtype =
+  |Add1
+  |Rem1
+  |Add2
+  |Rem2
+
+// apply an operation to a state
+let do (s:concrete_st) (o:op_t) : concrete_st =
+ match o with
+  |(_, (rid, Add1)) -> S.filter s (fun e -> snd e <> 1)
+  |(ts, (rid, Rem1)) -> S.add (ts, 1) s
+  |(_, (rid, Add2)) -> S.filter s (fun e -> snd e <> 2)
+  |(ts, (rid, Rem2)) -> S.add (ts, 2) s
+
+//conflict resolution
+let rc (o1 o2:op_t) =
+  match snd (snd o1), snd (snd o2) with
+  |Add1, Rem1 |Add2, Rem2 -> Fst_then_snd
+  |Rem1, Add1 | Rem2, Add2 -> Snd_then_fst
+  |_ -> Either
+
+// concrete merge operation
+let merge (l a b:concrete_st) : concrete_st =
+  let da = S.difference a l in
+  let db = S.difference b l in
+  let i_ab = S.intersection a b in
+  let i_lab = S.intersection l i_ab in
+  S.union i_lab (S.union da db)
+
+/////////////////////////////////////////////////////////////////////////////
+
+#set-options "--z3rlimit 300 --ifuel 3"
+let rc_non_comm_help1 (o1 o2:op_t)
+  : Lemma (requires distinct_ops o1 o2)
+          (ensures ((Add1? (snd (snd o1)) /\ Rem1? (snd (snd o2))) \/ (Rem1? (snd (snd o1)) /\ Add1? (snd (snd o2))))
+                           ==> ~ (eq (do (do init_st o1) o2) (do (do init_st o2) o1))) = ()
+         
+let rc_non_comm_help2 (o1 o2:op_t)
+  : Lemma (requires distinct_ops o1 o2)
+          (ensures ((Add2? (snd (snd o1)) /\ Rem2? (snd (snd o2))) \/ (Rem2? (snd (snd o1)) /\ Add2? (snd (snd o2))))
+                           ==> ~ (eq (do (do init_st o1) o2) (do (do init_st o2) o1))) = ()
+          
+let rc_non_comm (o1 o2:op_t)
+  : Lemma (requires distinct_ops o1 o2)
+          (ensures Either? (rc o1 o2) <==> commutes_with o1 o2) = 
+  rc_non_comm_help1 o1 o2;
+  rc_non_comm_help2 o1 o2
+
+let no_rc_chain (o1 o2 o3:op_t)
+  : Lemma (requires distinct_ops o1 o2 /\ distinct_ops o2 o3)
+          (ensures ~ (Fst_then_snd? (rc o1 o2) /\ Fst_then_snd? (rc o2 o3))) = ()
+
+let cond_comm_base (s:concrete_st) (o1 o2 o3:op_t) 
+  : Lemma (requires distinct_ops o1 o2 /\ distinct_ops o2 o3 /\ distinct_ops o1 o3 /\
+                    Fst_then_snd? (rc o1 o2) /\ ~ (Either? (rc o2 o3)))
+          (ensures eq (do (do (do s o1) o2) o3) (do (do (do s o2) o1) o3)) = ()
+
+let cond_comm_ind (s:concrete_st) (o1 o2 o3 o:op_t) (l:seq op_t)
+  : Lemma (requires distinct_ops o1 o2 /\ distinct_ops o1 o3 /\ distinct_ops o2 o3 /\ 
+                    Fst_then_snd? (rc o1 o2) /\ ~ (Either? (rc o2 o3)) /\
+                    eq (do (apply_log (do (do s o1) o2) l) o3) (do (apply_log (do (do s o2) o1) l) o3))
+          (ensures eq (do (do (apply_log (do (do s o1) o2) l) o) o3) (do (do (apply_log (do (do s o2) o1) l) o) o3)) = ()
+                   
+/////////////////////////////////////////////////////////////////////////////
+// Merge commutativity
+let merge_comm (l a b:concrete_st)
+   : Lemma (ensures (eq (merge l a b) (merge l b a))) = ()
+
+// Merge idempotence
+let merge_idem (s:concrete_st)
+   : Lemma (ensures eq (merge s s s) s) = ()
+
+let base_2op o1 o2 = ()
+
+let ind_lca_2op l o1 o2 ol = ()
+
+let inter_right_base_2op l a b o1 o2 ob ol = ()
+     
+let inter_left_base_2op l a b o1 o2 ob ol = ()
+
+let inter_right_2op l a b o1 o2 ob ol o = ()
+
+let inter_left_2op l a b o1 o2 ob ol o = ()
+
+let ind_right_2op l a b o1 o2 o2' = ()
+
+let ind_left_2op l a b o1 o2 o1' = ()
+
+let base_1op o1 = ()
+
+let ind_lca_1op l o1 ol = ()
+
+let inter_right_base_1op l a b o1 ob ol = ()
+     
+let inter_left_base_1op l a b o1 ob ol = ()
+   
+let inter_right_1op l a b o1 ob ol o = ()
+
+let inter_left_1op l a b o1 ob ol o = ()
+
+let ind_left_1op l a b o1 o1' ol = ()
+
+let ind_right_1op l a b o2 o2' ol = ()
+
+let lem_0op l a b ol = ()
